ConsistentInits.v
@@ -1,0 +1,362 @@
+From Elo Require Import Core.
+From Elo Require Import Properties1.
+
+From Elo Require Import NoUninitRefs.
+From Elo Require Import OneInit.
+From Elo Require Import UniqueInits.
+
+(* ------------------------------------------------------------------------- *)
+(* consistent-inits                                                          *)
+(* ------------------------------------------------------------------------- *)
+
+Inductive consistent_inits (m : mem) : tm -> Prop :=
+  | ci_unit  :                consistent_inits m <{unit         }> 
+  | ci_nat   : forall n,      consistent_inits m <{nat n        }>
+  | ci_var   : forall x,      consistent_inits m <{var x        }>
+  | ci_fun   : forall x Tx t, consistent_inits m t  ->
+                              consistent_inits m <{fn x Tx t    }>
+  | ci_call  : forall t1 t2,  consistent_inits m t1 ->
+                              consistent_inits m t2 ->
+                              consistent_inits m <{call t1 t2   }> 
+  | ci_ref   : forall ad T,   consistent_inits m <{&ad : T      }>
+
+  | ci_initR : forall ad t T, m[ad].t = None        ->
+                              m[ad].T = `r&T`       ->
+                              consistent_inits m t  ->
+                              consistent_inits m <{init ad t : r&T}> 
+
+  | ci_initX : forall ad t T, m[ad].t = None        ->
+                              m[ad].T = `x&T`       ->
+                              consistent_inits m t  ->
+                              consistent_inits m <{init ad t : x&T}> 
+
+  | ci_initW : forall ad t T, m[ad].t = None        ->
+                              m[ad].T = `w&T`       ->
+                              consistent_inits m t  ->
+                              consistent_inits m <{init ad t : w&T}> 
+
+  | ci_new   : forall T t,    consistent_inits m t  ->
+                              consistent_inits m <{new t : T    }> 
+  | ci_load  : forall t,      consistent_inits m t  ->
+                              consistent_inits m <{*t           }> 
+  | ci_asg   : forall t1 t2,  consistent_inits m t1 ->
+                              consistent_inits m t2 ->
+                              consistent_inits m <{t1 := t2     }> 
+  | ci_acq   : forall t1 t2,  consistent_inits m t1 ->
+                              consistent_inits m t2 ->
+                              consistent_inits m <{acq t1 t2    }>
+  | ci_cr    : forall ad t,   consistent_inits m t  ->
+                              consistent_inits m <{cr ad t      }>
+  | ci_spawn : forall t,      consistent_inits m t  ->
+                              consistent_inits m <{spawn t      }>
+  .
+
+(* inversion --------------------------------------------------------------- *)
+
+Local Ltac _ci tt :=
+  match goal with
+  | H : consistent_inits _ <{unit        }> |- _ => clear H
+  | H : consistent_inits _ <{nat _       }> |- _ => clear H
+  | H : consistent_inits _ <{var _       }> |- _ => clear H
+  | H : consistent_inits _ <{fn _ _ _    }> |- _ => tt H
+  | H : consistent_inits _ <{call _ _    }> |- _ => tt H
+  | H : consistent_inits _ <{& _ : _     }> |- _ => clear H
+  | H : consistent_inits _ <{new _ : _   }> |- _ => tt H
+  | H : consistent_inits _ <{init _ _ : _}> |- _ => tt H
+  | H : consistent_inits _ <{* _         }> |- _ => tt H
+  | H : consistent_inits _ <{_ := _      }> |- _ => tt H
+  | H : consistent_inits _ <{acq _ _     }> |- _ => tt H
+  | H : consistent_inits _ <{cr _ _      }> |- _ => tt H
+  | H : consistent_inits _ <{spawn _     }> |- _ => tt H
+  end.
+
+Ltac inv_ci  := _ci inv.
+Ltac invc_ci := _ci invc.
+
+(* theorems ---------------------------------------------------------------- *)
+
+Theorem insert_then_uninitialized : forall m ad t t1 t2,
+  consistent_inits m t1 ->
+  (* --- *)
+  t1 --[e_insert ad t]--> t2 ->
+  m[ad].t = None.
+Proof.
+  intros. ind_tstep; invc_ci; auto.
+Qed.
+
+(* lemmas ------------------------------------------------------------------ *)
+
+Lemma ci_from_noinits : forall m t,
+  no_inits t ->
+  consistent_inits m t.
+Proof.
+  intros. induction t; invc_noinits; eauto using consistent_inits.
+Qed.
+
+Lemma ci_insert_term : forall m t1 t2 ad t,
+  consistent_inits m t1 ->
+  t1 --[e_insert ad t]--> t2 ->
+  consistent_inits m t.
+Proof.
+  intros. ind_tstep; invc_ci; eauto.
+Qed.
+
+Lemma ci_write_term : forall m t1 t2 ad t,
+  consistent_inits m t1 ->
+  t1 --[e_write ad t]--> t2 ->
+  consistent_inits m t.
+Proof.
+  intros. ind_tstep; invc_ci; eauto.
+Qed.
+
+Local Corollary oneinit_from_ui : forall m ths tid t ad te,
+  forall_threads ths (valid_addresses m) ->
+  (* --- *)
+  unique_initializers m ths ->
+  ths[tid] --[e_insert ad te]--> t ->
+  one_init ad ths[tid].
+Proof.
+  intros * ? Hui ?.
+  assert (Had : ad < #m) by eauto using vad_insert_addr.
+  specialize (Hui ad Had) as [Hfall Hfone].
+  destruct (alt_opt_dec m[ad].t); aspecialize.
+  - specialize Hfone as [tid' [? ?]].
+    destruct (nat_eq_dec tid' tid); subst; trivial.
+    exfalso. eauto using noinit_insert_contradiction.
+  - exfalso. eauto using noinit_insert_contradiction.
+Qed.
+
+Local Corollary noinit_from_ui : forall m ths tid1 tid2 ad,
+  forall_threads ths (valid_addresses m) ->
+  unique_initializers m ths ->
+  (* --- *)
+  tid1 <> tid2 ->
+  one_init ad ths[tid1] ->
+  no_init ad ths[tid2].
+Proof.
+  intros * ? Hui ? **.
+  assert (Had : ad < #m) by eauto using oneinit_ad_bound.
+  specialize (Hui ad Had) as [Hfall Hfone].
+  destruct (alt_opt_dec m[ad].t); aspecialize.
+  - specialize Hfone as [tid' [? ?]].
+    destruct (nat_eq_dec tid1 tid'); subst;
+    eauto using noinit_oneinit_contradiction.
+  - eauto using noinit_oneinit_contradiction.
+Qed.
+
+(* preservation ------------------------------------------------------------ *)
+
+Lemma ci_subst : forall m x tx t,
+  consistent_inits m t ->
+  consistent_inits m tx ->
+  consistent_inits m <{[x := tx] t}>.
+Proof.
+  intros. induction t; invc_ci; simpl;
+  try destruct str_eq_dec; eauto using consistent_inits.
+Qed.
+
+Lemma ci_mem_add : forall m t c,
+  valid_addresses m t ->
+  (* --- *)
+  consistent_inits m t ->
+  consistent_inits (m +++ c) t.
+Proof.
+  intros. induction t; invc_vad; invc_ci;
+  constructor; sigma; eauto using consistent_inits.
+Qed.
+
+Lemma ci_mem_set1 : forall m t t' ad,
+  no_init ad t ->
+  (* --- *)
+  consistent_inits m t' ->
+  consistent_inits m t  ->
+  consistent_inits m[ad.t <- t'] t.
+Proof.
+  intros. induction t; invc_noinit; invc_ci;
+  constructor; sigma; eauto.
+Qed.
+
+Lemma ci_mem_set2 : forall m t t' ad,
+  no_inits t ->
+  no_inits t' ->
+  consistent_inits m[ad.t <- t'] t.
+Proof.
+  intros. induction t; invc_noinits; eauto using consistent_inits.
+Qed.
+
+Lemma ci_mem_acq : forall m t ad,
+  consistent_inits m t ->
+  consistent_inits m[ad.X <- true] t.
+Proof.
+  intros. induction t; invc_ci; constructor; upsilon; eauto.
+Qed.
+
+Lemma ci_mem_rel : forall m t ad,
+  consistent_inits m t ->
+  consistent_inits m[ad.X <- false] t.
+Proof.
+  intros. induction t; invc_ci; constructor; upsilon; eauto.
+Qed.
+
+(* ------------------------------------------------------------------------- *)
+
+Lemma ci_preservation_none : forall m t1 t2,
+  consistent_inits m t1 ->
+  t1 --[e_none]--> t2 ->
+  consistent_inits m t2.
+Proof.
+  intros. ind_tstep; repeat invc_ci; eauto using ci_subst, consistent_inits.
+Qed.
+
+Lemma ci_preservation_alloc : forall m t1 t2 T,
+  valid_addresses m t1 ->
+  well_typed_term t1 ->
+  (* --- *)
+  consistent_inits m t1 ->
+  t1 --[e_alloc (#m) T]--> t2 ->
+  consistent_inits (m +++ (None, T, false)) t2.
+Proof.
+  intros * ? [T ?] **. gendep T.
+  ind_tstep; intros; invc_vad; invc_typeof; invc_ci;
+  constructor; sigma; eauto using ci_mem_add.
+Qed.
+
+Lemma ci_preservation_insert : forall m t1 t2 ad t,
+  one_init ad t1 ->
+  (* --- *)
+  consistent_inits m t1 ->
+  t1 --[e_insert ad t]--> t2 ->
+  consistent_inits m[ad.t <- t] t2.
+Proof.
+  intros. assert (consistent_inits m t) by eauto using ci_insert_term.
+  ind_tstep; invc_oneinit; invc_ci;
+  constructor; sigma; eauto using ci_mem_set1;
+  exfalso; eauto using noinit_insert_contradiction.
+Qed.
+
+Lemma ci_preservation_read : forall m t1 t2 ad t,
+  consistent_inits m t ->
+  (* --- *)
+  consistent_inits m t1 ->
+  t1 --[e_read ad t]--> t2 ->
+  consistent_inits m t2.
+Proof.
+  intros. ind_tstep; invc_ci; eauto using consistent_inits.
+Qed.
+
+Lemma ci_preservation_write : forall m t1 t2 ad t,
+  no_init ad t1 ->
+  (* --- *)
+  consistent_inits m t1 ->
+  t1 --[e_write ad t]--> t2 ->
+  consistent_inits m[ad.t <- t] t2.
+Proof.
+  intros. ind_tstep; invc_noinit; invc_ci;
+  eauto using consistent_inits;
+  constructor; sigma; eauto using ci_write_term, ci_mem_set1.
+Qed.
+
+Lemma ci_preservation_acq : forall m t1 t2 ad t,
+  consistent_inits m t ->
+  (* --- *)
+  consistent_inits m t1 ->
+  t1 --[e_acq ad t]--> t2 ->
+  consistent_inits m[ad.X <- true] t2.
+Proof.
+  intros. eapply ci_mem_acq. ind_tstep; repeat invc_ci;
+  eauto using ci_subst, consistent_inits.
+Qed.
+
+Lemma ci_preservation_rel : forall m t1 t2 ad,
+  consistent_inits m t1 ->
+  t1 --[e_rel ad]--> t2 ->
+  consistent_inits m[ad.X <- false] t2.
+Proof.
+  intros. eapply ci_mem_rel. ind_tstep; repeat invc_ci;
+  eauto using consistent_inits.
+Qed.
+
+Lemma ci_preservation_spawn : forall m t1 t2 tid t,
+  consistent_inits m t1 ->
+  t1 --[e_spawn tid t]--> t2 ->
+  consistent_inits m t2.
+Proof.
+  intros. ind_tstep; invc_ci; eauto using consistent_inits.
+Qed.
+
+Lemma ci_preservation_spawned : forall m t1 t2 tid t,
+  consistent_inits m t1 ->
+  t1 --[e_spawn tid t]--> t2 ->
+  consistent_inits m t.
+Proof.
+  intros. ind_tstep; invc_ci; eauto using consistent_inits.
+Qed.
+
+Theorem ci_preservation_ths : forall m1 m2 ths1 ths2 tid e,
+  forall_program m1 ths1 (valid_addresses m1) ->
+  forall_program m1 ths1 valid_blocks ->
+  forall_program m1 ths1 well_typed_term ->
+  no_uninitialized_references m1 ths1 ->
+  unique_initializers m1 ths1 ->
+  (* --- *)
+  forall_program m1 ths1 (consistent_inits m1) ->
+  m1 / ths1 ~~[tid, e]~~> m2 / ths2 ->
+  forall_threads ths2 (consistent_inits m2).
+Proof.
+  intros * [? ?] [? ?] [? ?] ? Hui [? ?] ?.
+  invc_cstep; try invc_mstep; upsilon; intros.
+  - eauto using ci_preservation_none.
+  - eauto using ci_preservation_alloc.
+  - eauto using ci_mem_add.
+  - assert (one_init ad ths1[tid]) by eauto using oneinit_from_ui.
+    eauto using ci_preservation_insert.
+  - assert (one_init ad ths1[tid] ) by eauto using oneinit_from_ui.
+    assert (no_init  ad ths1[tid']) by eauto using noinit_from_ui.
+    eapply ci_mem_set1; eauto using ci_from_noinits,
+      vb_insert_term, value_insert_term, noinits_from_value.
+  - eauto using ci_preservation_read.
+  - assert (m1[ad].t <> None) by eauto using write_then_initialized. 
+    specialize (Hui ad) as [Hnoinit _]; trivial. aspecialize.
+    eauto using ci_preservation_write.
+  - assert (m1[ad].t <> None) by eauto using write_then_initialized. 
+    specialize (Hui ad) as [Hnoinit _]; trivial. aspecialize.
+    eauto using ci_write_term, ci_mem_set1.
+  - eauto using ci_preservation_acq.
+  - eauto using ci_mem_acq.
+  - eauto using ci_preservation_rel.
+  - eauto using ci_mem_rel.
+  - eauto using ci_preservation_spawn.
+  - eauto using ci_preservation_spawned.
+Qed.
+
+Corollary ci_preservation_mem : forall m1 m2 ths1 ths2 tid e,
+  forall_memory  m1 value ->
+  forall_program m1 ths1 valid_blocks ->
+  (* --- *)
+  m1 / ths1 ~~[tid, e]~~> m2 / ths2 ->
+  forall_memory m2 (consistent_inits m2).
+Proof.
+  intros ** ? ? ?.
+  assert (forall_memory m2 value)
+    by eauto using value_preservation.
+  assert (forall_program m2 ths2 valid_blocks) as [? _]
+    by eauto using vb_preservation.
+  eauto using noinits_from_value, ci_from_noinits.
+Qed.
+
+Theorem ci_preservation : forall m1 m2 ths1 ths2 tid e,
+  forall_memory  m1 value ->
+  forall_program m1 ths1 (valid_addresses m1) ->
+  forall_program m1 ths1 valid_blocks ->
+  forall_program m1 ths1 well_typed_term ->
+  no_uninitialized_references m1 ths1 ->
+  unique_initializers m1 ths1 ->
+  (* --- *)
+  forall_program m1 ths1 (consistent_inits m1) ->
+  m1 / ths1 ~~[tid, e]~~> m2 / ths2 ->
+  forall_program m2 ths2 (consistent_inits m2).
+Proof.
+  intros until 6. intros Hci **. split;
+  eauto using ci_preservation_mem, ci_preservation_ths.
+Qed.
+
