Inheritance1.v
@@ -1,0 +1,164 @@
+From Elo Require Import Core.
+
+From Elo Require Import NoInit.
+From Elo Require Import NoCR.
+From Elo Require Import ValidBlocks.
+
+(* ------------------------------------------------------------------------- *)
+(* no-init inheritance                                                       *)
+(* ------------------------------------------------------------------------- *)
+
+Local Lemma noinit_inheritance_subst : forall x Tx t tx ad,
+  no_init ad tx ->
+  no_init ad <{[x := tx] t}> ->
+  no_init ad <{call <{fn x Tx t}> tx}>.
+Proof.
+  intros. repeat constructor; trivial.
+  induction t; simpl in *;
+  try destruct str_eq_dec; try invc_noinit; eauto using no_init.
+Qed.
+
+(* ------------------------------------------------------------------------- *)
+
+Local Ltac solve_noinit_inheritance :=
+  intros; ind_tstep; repeat invc_vb; try invc_noinit;
+  eauto using noinit_from_value, noinit_inheritance_subst, no_init.
+
+Lemma noinit_inheritance_none : forall ad t1 t2,
+  valid_blocks t1 ->
+  (* --- *)
+  no_init ad t2 ->
+  t1 --[e_none]--> t2 ->
+  no_init ad t1.
+Proof. solve_noinit_inheritance. Qed.
+
+Lemma noinit_inheritance_alloc : forall ad ad' t1 t2 T,
+  no_init ad t2 ->
+  t1 --[e_alloc ad' T]--> t2 ->
+  no_init ad t1.
+Proof. solve_noinit_inheritance. Qed.
+
+Lemma noinit_inheritance_insert : forall ad ad' t t1 t2,
+  valid_blocks t1 ->
+  (* --- *)
+  ad <> ad' ->
+  no_init ad t2 ->
+  t1 --[e_insert ad' t]--> t2 ->
+  no_init ad t1.
+Proof. solve_noinit_inheritance. Qed.
+
+Lemma noinit_inheritance_read : forall ad ad' t t1 t2,
+  no_init ad t2 ->
+  t1 --[e_read ad' t]--> t2 ->
+  no_init ad t1.
+Proof. solve_noinit_inheritance. Qed.
+
+Lemma noinit_inheritance_write : forall ad ad' t t1 t2,
+  valid_blocks t1 ->
+  (* --- *)
+  no_init ad t2 ->
+  t1 --[e_write ad' t]--> t2 ->
+  no_init ad t1.
+Proof. solve_noinit_inheritance. Qed.
+
+Lemma noinit_inheritance_acq : forall ad ad' t t1 t2,
+  valid_blocks t1 ->
+  (* --- *)
+  no_init ad t2 ->
+  t1 --[e_acq ad' t]--> t2 ->
+  no_init ad t1.
+Proof. solve_noinit_inheritance. Qed.
+
+Lemma noinit_inheritance_rel : forall ad ad' t1 t2,
+  no_init ad t2 ->
+  t1 --[e_rel ad']--> t2 ->
+  no_init ad t1.
+Proof. solve_noinit_inheritance. Qed.
+
+Lemma noinit_inheritance_spawn : forall ad tid t t1 t2,
+  valid_blocks t1 ->
+  (* --- *)
+  no_init ad t2 ->
+  t1 --[e_spawn tid t]--> t2 ->
+  no_init ad t1.
+Proof. solve_noinit_inheritance. Qed.
+
+(* ------------------------------------------------------------------------- *)
+(* no-cr inheritance                                                         *)
+(* ------------------------------------------------------------------------- *)
+
+Local Lemma nocr_inheritance_subst : forall x Tx t tx ad,
+  no_cr ad tx ->
+  no_cr ad <{[x := tx] t}> ->
+  no_cr ad <{call <{fn x Tx t}> tx}>.
+Proof.
+  intros. repeat constructor; trivial.
+  induction t; simpl in *;
+  try destruct str_eq_dec; try invc_nocr; eauto using no_cr.
+Qed.
+
+(* ------------------------------------------------------------------------- *)
+
+Local Ltac solve_nocr_inheritance :=
+  intros; ind_tstep; repeat invc_vb; try invc_nocr;
+  eauto using nocr_from_value, nocr_inheritance_subst, no_cr.
+
+Lemma nocr_inheritance_none : forall ad t1 t2,
+  valid_blocks t1 ->
+  (* --- *)
+  no_cr ad t2 ->
+  t1 --[e_none]--> t2 ->
+  no_cr ad t1.
+Proof. solve_nocr_inheritance. Qed.
+
+Lemma nocr_inheritance_alloc : forall ad ad' t1 t2 T,
+  no_cr ad t2 ->
+  t1 --[e_alloc ad' T]--> t2 ->
+  no_cr ad t1.
+Proof. solve_nocr_inheritance. Qed.
+
+Lemma nocr_inheritance_insert : forall ad ad' t t1 t2,
+  valid_blocks t1 ->
+  (* --- *)
+  no_cr ad t2 ->
+  t1 --[e_insert ad' t]--> t2 ->
+  no_cr ad t1.
+Proof. solve_nocr_inheritance. Qed.
+
+Lemma nocr_inheritance_read : forall ad ad' t t1 t2,
+  no_cr ad t2 ->
+  t1 --[e_read ad' t]--> t2 ->
+  no_cr ad t1.
+Proof. solve_nocr_inheritance. Qed.
+
+Lemma nocr_inheritance_write : forall ad ad' t t1 t2,
+  valid_blocks t1 ->
+  (* --- *)
+  no_cr ad t2 ->
+  t1 --[e_write ad' t]--> t2 ->
+  no_cr ad t1.
+Proof. solve_nocr_inheritance. Qed.
+
+Lemma nocr_inheritance_acq : forall ad ad' t t1 t2,
+  valid_blocks t1 ->
+  (* --- *)
+  no_cr ad t2 ->
+  t1 --[e_acq ad' t]--> t2 ->
+  no_cr ad t1.
+Proof. solve_nocr_inheritance. Qed.
+
+Lemma nocr_inheritance_rel : forall ad ad' t1 t2,
+  ad <> ad' ->
+  no_cr ad t2 ->
+  t1 --[e_rel ad']--> t2 ->
+  no_cr ad t1.
+Proof. solve_nocr_inheritance. Qed.
+
+Lemma nocr_inheritance_spawn : forall ad tid t t1 t2,
+  valid_blocks t1 ->
+  (* --- *)
+  no_cr ad t2 ->
+  t1 --[e_spawn tid t]--> t2 ->
+  no_cr ad t1.
+Proof. solve_nocr_inheritance. Qed.
+
