NoCR.v
@@ -1,0 +1,238 @@
+From Elo Require Import Core.
+
+From Elo Require Import ValidAddresses.
+
+(* ------------------------------------------------------------------------- *)
+(* no-cr                                                                     *)
+(* ------------------------------------------------------------------------- *)
+
+Inductive no_cr (ad : addr) : tm -> Prop :=
+  | nocr_unit  :                 no_cr ad <{unit          }>
+  | nocr_nat   : forall n,       no_cr ad <{nat n         }>
+  | nocr_var   : forall x,       no_cr ad <{var x         }>
+  | nocr_fun   : forall x Tx t,  no_cr ad t  ->
+                                 no_cr ad <{fn x Tx t     }>
+  | nocr_call  : forall t1 t2,   no_cr ad t1 ->
+                                 no_cr ad t2 ->
+                                 no_cr ad <{call t1 t2    }>
+  | nocr_ref   : forall ad' T,   no_cr ad <{&ad' : T      }>
+  | nocr_new   : forall t T,     no_cr ad t  ->
+                                 no_cr ad <{new t : T     }>
+  | nocr_init  : forall ad' t T, no_cr ad t  ->
+                                 no_cr ad <{init ad' t : T}>
+  | nocr_load  : forall t,       no_cr ad t  ->
+                                 no_cr ad <{*t            }>
+  | nocr_asg   : forall t1 t2,   no_cr ad t1 ->
+                                 no_cr ad t2 ->
+                                 no_cr ad <{t1 := t2      }>
+  | nocr_acq   : forall t1 t2,   no_cr ad t1 ->
+                                 no_cr ad t2 ->
+                                 no_cr ad <{acq t1 t2     }>
+  | nocr_cr    : forall ad' t,   ad <> ad'   ->
+                                 no_cr ad t  ->
+                                 no_cr ad <{cr ad' t      }>
+  | nocr_spawn : forall t,       no_cr ad t  ->
+                                 no_cr ad <{spawn t       }>
+  .
+
+(* inversion --------------------------------------------------------------- *)
+
+Local Ltac _nocr tt :=
+  match goal with
+  | H : no_cr _   <{unit        }> |- _ => clear H
+  | H : no_cr _   <{nat _       }> |- _ => clear H
+  | H : no_cr _   <{var _       }> |- _ => clear H
+  | H : no_cr _   <{fn _ _ _    }> |- _ => tt H
+  | H : no_cr _   <{call _ _    }> |- _ => tt H
+  | H : no_cr _   <{&_ : _      }> |- _ => clear H
+  | H : no_cr _   <{new _ : _   }> |- _ => tt H
+  | H : no_cr _   <{init _ _ : _}> |- _ => tt H
+  | H : no_cr _   <{* _         }> |- _ => tt H
+  | H : no_cr _   <{_ := _      }> |- _ => tt H
+  | H : no_cr _   <{acq _ _     }> |- _ => tt H
+  | H : no_cr ?ad <{cr ?ad _    }> |- _ => invc H; eauto
+  | H : no_cr _   <{cr _ _      }> |- _ => tt H
+  | H : no_cr _   <{spawn _     }> |- _ => tt H
+  end.
+
+Ltac inv_nocr  := _nocr inv.
+Ltac invc_nocr := _nocr invc.
+
+(* lemmas ------------------------------------------------------------------ *)
+
+Lemma nocr_rel_contradiction : forall t1 t2 ad,
+  no_cr ad t1 ->
+  t1 --[e_rel ad]--> t2 ->
+  False.
+Proof.
+  intros. ind_tstep; invc_nocr; auto.
+Qed.
+
+Lemma nocr_from_vad : forall m t,
+  valid_addresses m t ->
+  no_cr (#m) t.
+Proof.
+  intros. induction t; invc_vad; auto using no_cr.
+Qed.
+
+(* preservation lemmas ----------------------------------------------------- *)
+
+Lemma nocr_subst : forall ad x tx t,
+  no_cr ad t ->
+  no_cr ad tx ->
+  no_cr ad <{[x := tx] t}>.
+Proof.
+  intros. induction t; simpl in *; trivial;
+  try (destruct str_eq_dec; subst); trivial;
+  invc_nocr; eauto using no_cr.
+Qed.
+
+(* preservation ------------------------------------------------------------ *)
+
+Local Ltac solve_nocr_preservation :=
+  intros; ind_tstep; repeat invc_nocr; eauto using nocr_subst, no_cr.
+
+Lemma nocr_preservation_none : forall t1 t2 ad,
+  no_cr ad t1 ->
+  t1 --[e_none]--> t2 ->
+  no_cr ad t2.
+Proof. solve_nocr_preservation. Qed.
+
+Lemma nocr_preservation_alloc : forall t1 t2 ad ad' T,
+  no_cr ad t1 ->
+  t1 --[e_alloc ad' T]--> t2 ->
+  no_cr ad t2.
+Proof. solve_nocr_preservation. Qed.
+
+Lemma nocr_preservation_insert : forall t1 t2 ad ad' t,
+  no_cr ad t1 ->
+  t1 --[e_insert ad' t]--> t2 ->
+  no_cr ad t2.
+Proof. solve_nocr_preservation. Qed.
+
+Lemma nocr_preservation_read : forall t1 t2 ad ad' t,
+  no_cr ad t ->
+  (* --- *)
+  no_cr ad t1 ->
+  t1 --[e_read ad' t]--> t2 ->
+  no_cr ad t2.
+Proof. solve_nocr_preservation. Qed.
+
+Lemma nocr_preservation_write : forall t1 t2 ad ad' t,
+  no_cr ad t1 ->
+  t1 --[e_write ad' t]--> t2 ->
+  no_cr ad t2.
+Proof. solve_nocr_preservation. Qed.
+
+Lemma nocr_preservation_acq : forall t1 t2 ad ad' t,
+  no_cr ad t ->
+  (* --- *)
+  ad <> ad' ->
+  no_cr ad t1 ->
+  t1 --[e_acq ad' t]--> t2 ->
+  no_cr ad t2.
+Proof. solve_nocr_preservation. Qed.
+
+Lemma nocr_preservation_rel : forall t1 t2 ad ad',
+  ad <> ad' ->
+  no_cr ad' t1 ->
+  t1 --[e_rel ad]--> t2 ->
+  no_cr ad' t2.
+Proof. solve_nocr_preservation. Qed.
+
+Lemma nocr_preservation_spawn : forall t1 t2 ad tid t,
+  no_cr ad t1 ->
+  t1 --[e_spawn tid t]--> t2 ->
+  no_cr ad t2.
+Proof. solve_nocr_preservation. Qed.
+
+Lemma nocr_preservation_spawned : forall t1 t2 ad tid t,
+  no_cr ad t1 ->
+  t1 --[e_spawn tid t]--> t2 ->
+  no_cr ad t.
+Proof. solve_nocr_preservation. Qed.
+
+(* ------------------------------------------------------------------------- *)
+(* no-crs                                                                    *)
+(* ------------------------------------------------------------------------- *)
+
+Definition no_crs (t : tm) := forall ad, no_cr ad t.
+
+(* inversion --------------------------------------------------------------- *)
+
+Local Ltac solve_inv_nocrs :=
+  unfold no_crs; intros * H; try split;
+  intros **; auto_specialize; invc_nocr; eauto.
+
+Local Lemma inv_nocrs_fun : forall x Tx t,
+  no_crs <{fn x Tx t}> -> no_crs t.
+Proof. solve_inv_nocrs. Qed.
+
+Local Lemma inv_nocrs_call : forall t1 t2,
+  no_crs <{call t1 t2}> -> no_crs t1 /\ no_crs t2.
+Proof. solve_inv_nocrs. Qed.
+
+Local Lemma inv_nocrs_new : forall t T,
+  no_crs <{new t : T}> -> no_crs t.
+Proof. solve_inv_nocrs. Qed.
+
+Local Lemma inv_nocrs_init : forall ad t T,
+  no_crs <{init ad t : T}> -> no_crs t.
+Proof. solve_inv_nocrs. Qed.
+
+Local Lemma inv_nocrs_load : forall t,
+  no_crs <{*t}> -> no_crs t.
+Proof. solve_inv_nocrs. Qed.
+
+Local Lemma inv_nocrs_asg : forall t1 t2,
+  no_crs <{t1 := t2}> -> no_crs t1 /\ no_crs t2.
+Proof. solve_inv_nocrs. Qed.
+
+Local Lemma inv_nocrs_acq : forall t1 t2,
+  no_crs <{acq t1 t2}> -> no_crs t1 /\ no_crs t2.
+Proof. solve_inv_nocrs. Qed.
+
+Local Lemma inv_nocrs_cr : forall ad t,
+  no_crs <{cr ad t}> -> False.
+Proof. solve_inv_nocrs. Qed.
+
+Local Lemma inv_nocrs_spawn : forall t,
+  no_crs <{spawn t}> -> no_crs t.
+Proof. solve_inv_nocrs. Qed.
+
+Ltac invc_nocrs :=
+  match goal with
+  | H : no_crs <{unit        }> |- _ => clear H
+  | H : no_crs <{nat _       }> |- _ => clear H
+  | H : no_crs <{var _       }> |- _ => clear H
+  | H : no_crs <{fn _ _ _    }> |- _ => eapply inv_nocrs_fun    in H
+  | H : no_crs <{call _ _    }> |- _ => eapply inv_nocrs_call   in H as [? ?]
+  | H : no_crs <{& _ : _     }> |- _ => clear H
+  | H : no_crs <{new _ : _   }> |- _ => eapply inv_nocrs_new    in H
+  | H : no_crs <{init _ _ : _}> |- _ => eapply inv_nocrs_init   in H
+  | H : no_crs <{* _         }> |- _ => eapply inv_nocrs_load   in H
+  | H : no_crs <{_ := _      }> |- _ => eapply inv_nocrs_asg    in H as [? ?]
+  | H : no_crs <{acq _ _     }> |- _ => eapply inv_nocrs_acq    in H as [? ?]
+  | H : no_crs <{cr _ _      }> |- _ => eapply inv_nocrs_cr     in H; eauto
+  | H : no_crs <{spawn _     }> |- _ => eapply inv_nocrs_spawn  in H
+  end.
+
+(* lemmas ------------------------------------------------------------------ *)
+
+Corollary nocr_from_nocrs : forall ad t,
+  no_crs t ->
+  no_cr ad t.
+Proof.
+  unfold no_crs. auto.
+Qed.
+
+(* preservation lemmas ----------------------------------------------------- *)
+
+Corollary nocrs_subst : forall x tx t,
+  no_crs t ->
+  no_crs tx ->
+  no_crs <{[x := tx] t}>.
+Proof.
+  intros ** ?. eauto using nocr_subst.
+Qed.
+
