NoInit.v
@@ -1,0 +1,268 @@
+From Elo Require Import Core.
+
+From Elo Require Import ValidAddresses.
+
+(* ------------------------------------------------------------------------- *)
+(* no-init                                                                   *)
+(* ------------------------------------------------------------------------- *)
+
+Inductive no_init (ad : addr) : tm -> Prop :=
+  | noinit_unit  :                 no_init ad <{unit          }>
+  | noinit_nat   : forall n,       no_init ad <{nat n         }>
+  | noinit_var   : forall x,       no_init ad <{var x         }>
+  | noinit_fun   : forall x Tx t,  no_init ad t  ->
+                                   no_init ad <{fn x Tx t     }>
+  | noinit_call  : forall t1 t2,   no_init ad t1 ->
+                                   no_init ad t2 ->
+                                   no_init ad <{call t1 t2    }>
+  | noinit_ref   : forall ad' T,   no_init ad <{&ad' : T      }>
+  | noinit_new   : forall T t,     no_init ad t  ->
+                                   no_init ad <{new t : T     }>
+  | noinit_init  : forall ad' T t, ad <> ad'     ->
+                                   no_init ad t  ->
+                                   no_init ad <{init ad' t : T}>
+  | noinit_load  : forall t,       no_init ad t  ->
+                                   no_init ad <{*t            }>
+  | noinit_asg   : forall t1 t2,   no_init ad t1 ->
+                                   no_init ad t2 ->
+                                   no_init ad <{t1 := t2      }>
+  | noinit_acq   : forall t1 t2,   no_init ad t1 ->
+                                   no_init ad t2 ->
+                                   no_init ad <{acq t1 t2     }>
+  | noinit_cr    : forall ad' t,   no_init ad t  ->
+                                   no_init ad <{cr ad' t      }>
+  | noinit_spawn : forall t,       no_init ad t  ->
+                                   no_init ad <{spawn t       }>
+  .
+
+(* inversion --------------------------------------------------------------- *)
+
+Local Ltac _noinit tt :=
+  match goal with
+  | H : no_init _   <{unit          }> |- _ => clear H
+  | H : no_init _   <{nat _         }> |- _ => clear H
+  | H : no_init _   <{var _         }> |- _ => clear H
+  | H : no_init _   <{fn _ _ _      }> |- _ => tt H
+  | H : no_init _   <{call _ _      }> |- _ => tt H
+  | H : no_init _   <{&_ : _        }> |- _ => clear H
+  | H : no_init _   <{new _ : _     }> |- _ => tt H
+  | H : no_init ?ad <{init ?ad _ : _}> |- _ => invc H; eauto
+  | H : no_init _   <{init _ _ : _  }> |- _ => tt H
+  | H : no_init _   <{* _           }> |- _ => tt H
+  | H : no_init _   <{_ := _        }> |- _ => tt H
+  | H : no_init _   <{acq _ _       }> |- _ => tt H
+  | H : no_init _   <{cr _ _        }> |- _ => tt H
+  | H : no_init _   <{spawn _       }> |- _ => tt H
+  end.
+
+Ltac inv_noinit  := _noinit inv.
+Ltac invc_noinit := _noinit invc.
+
+(* lemmas ------------------------------------------------------------------ *)
+
+Lemma noinit_insert_term : forall t1 t2 ad ad' t,
+  no_init ad' t1 ->
+  t1 --[e_insert ad t]--> t2 ->
+  no_init ad' t.
+Proof.
+  intros. ind_tstep; invc_noinit; eauto using no_init.
+Qed.
+
+Lemma noinit_write_term : forall t1 t2 ad ad' t,
+  no_init ad' t1 ->
+  t1 --[e_write ad t]--> t2 ->
+  no_init ad' t.
+Proof.
+  intros. ind_tstep; invc_noinit; eauto using no_init.
+Qed.
+
+Lemma noinit_insert_contradiction : forall t1 t2 ad t,
+  no_init ad t1 ->
+  t1 --[e_insert ad t]--> t2 ->
+  False.
+Proof.
+  intros. ind_tstep; invc_noinit; eauto.
+Qed.
+
+Lemma noinit_from_vad : forall m t,
+  valid_addresses m t ->
+  no_init (#m) t.
+Proof.
+  intros. induction t; invc_vad; auto using no_init.
+Qed.
+
+(* preservation lemmas ----------------------------------------------------- *)
+
+Lemma noinit_subst : forall ad x tx t,
+  no_init ad t ->
+  no_init ad tx ->
+  no_init ad <{[x := tx] t}>.
+Proof.
+  intros. induction t; invc_noinit;
+  simpl in *; try destruct str_eq_dec; eauto using no_init.
+Qed.
+
+(* preservation ------------------------------------------------------------ *)
+
+Local Ltac solve_noinit_preservation :=
+  intros; ind_tstep; repeat invc_noinit; eauto using noinit_subst, no_init.
+
+Lemma noinit_preservation_none : forall ad t1 t2,
+  no_init ad t1 ->
+  t1 --[e_none]--> t2 ->
+  no_init ad t2.
+Proof. solve_noinit_preservation. Qed.
+
+Lemma noinit_preservation_alloc : forall ad t1 t2 ad' T,
+  ad <> ad' ->
+  no_init ad t1 ->
+  t1 --[e_alloc ad' T]--> t2 ->
+  no_init ad t2.
+Proof. solve_noinit_preservation. Qed.
+
+Lemma noinit_preservation_insert : forall ad t1 t2 ad' t,
+  ad <> ad' ->
+  no_init ad t1 ->
+  t1 --[e_insert ad' t]--> t2 ->
+  no_init ad t2.
+Proof. solve_noinit_preservation. Qed.
+
+Lemma noinit_preservation_read : forall ad t1 t2 ad' t,
+  no_init ad t ->
+  (* --- *)
+  no_init ad t1 ->
+  t1 --[e_read ad' t]--> t2 ->
+  no_init ad t2.
+Proof. solve_noinit_preservation. Qed.
+
+Lemma noinit_preservation_write : forall ad t1 t2 ad' t,
+  no_init ad t1 ->
+  t1 --[e_write ad' t]--> t2 ->
+  no_init ad t2.
+Proof. solve_noinit_preservation. Qed.
+
+Lemma noinit_preservation_acq : forall ad t1 t2 ad' t,
+  no_init ad t ->
+  (* --- *)
+  no_init ad t1 ->
+  t1 --[e_acq ad' t]--> t2 ->
+  no_init ad t2.
+Proof. solve_noinit_preservation. Qed.
+
+Lemma noinit_preservation_rel : forall ad t1 t2 ad',
+  no_init ad t1 ->
+  t1 --[e_rel ad']--> t2 ->
+  no_init ad t2.
+Proof. solve_noinit_preservation. Qed.
+
+Lemma noinit_preservation_spawn : forall ad t1 t2 tid t,
+  no_init ad t1 ->
+  t1 --[e_spawn tid t]--> t2 ->
+  no_init ad t2.
+Proof. solve_noinit_preservation. Qed.
+
+Lemma noinit_preservation_spawned : forall ad t1 t2 tid t,
+  no_init ad t1 ->
+  t1 --[e_spawn tid t]--> t2 ->
+  no_init ad t.
+Proof. solve_noinit_preservation. Qed.
+
+(* ------------------------------------------------------------------------- *)
+(* no-inits                                                                  *)
+(* ------------------------------------------------------------------------- *)
+
+Definition no_inits (t : tm) := forall ad, no_init ad t.
+
+(* inversion --------------------------------------------------------------- *)
+
+Local Ltac solve_inv_noinits :=
+  unfold no_inits; intros; try split; intros; aspecialize; invc_noinit; eauto.
+
+Local Lemma inv_noinits_fun : forall x Tx t,
+  no_inits <{fn x Tx t}> -> no_inits t.
+Proof. solve_inv_noinits. Qed.
+
+Local Lemma inv_noinits_call : forall t1 t2,
+  no_inits <{call t1 t2}> -> no_inits t1 /\ no_inits t2.
+Proof. solve_inv_noinits. Qed.
+
+Local Lemma inv_noinits_new : forall t T,
+  no_inits <{new t : T}> -> no_inits t.
+Proof. solve_inv_noinits. Qed.
+
+Local Lemma inv_noinits_init : forall ad t T,
+  no_inits <{init ad t : T}> -> False.
+Proof. solve_inv_noinits. Qed.
+
+Local Lemma inv_noinits_load : forall t,
+  no_inits <{*t}> -> no_inits t.
+Proof. solve_inv_noinits. Qed.
+
+Local Lemma inv_noinits_asg : forall t1 t2,
+  no_inits <{t1 := t2}> -> no_inits t1 /\ no_inits t2.
+Proof. solve_inv_noinits. Qed.
+
+Local Lemma inv_noinits_acq : forall t1 t2,
+  no_inits <{acq t1 t2}> -> no_inits t1 /\ no_inits t2.
+Proof. solve_inv_noinits. Qed.
+
+Local Lemma inv_noinits_cr : forall ad t,
+  no_inits <{cr ad t}> -> no_inits t.
+Proof. solve_inv_noinits. Qed.
+
+Local Lemma inv_noinits_spawn : forall t,
+  no_inits <{spawn t}> -> no_inits t.
+Proof. solve_inv_noinits. Qed.
+
+Ltac invc_noinits :=
+  match goal with
+  | H : no_inits <{unit        }> |- _ => clear H
+  | H : no_inits <{nat _       }> |- _ => clear H
+  | H : no_inits <{var _       }> |- _ => clear H
+  | H : no_inits <{fn _ _ _    }> |- _ => eapply inv_noinits_fun   in H
+  | H : no_inits <{call _ _    }> |- _ => eapply inv_noinits_call  in H as [? ?]
+  | H : no_inits <{& _ : _     }> |- _ => clear H
+  | H : no_inits <{new _ : _   }> |- _ => eapply inv_noinits_new   in H
+  | H : no_inits <{init _ _ : _}> |- _ => eapply inv_noinits_init  in H; eauto
+  | H : no_inits <{* _         }> |- _ => eapply inv_noinits_load  in H
+  | H : no_inits <{_ := _      }> |- _ => eapply inv_noinits_asg   in H as [? ?]
+  | H : no_inits <{acq _ _     }> |- _ => eapply inv_noinits_acq   in H as [? ?]
+  | H : no_inits <{cr _ _      }> |- _ => eapply inv_noinits_cr    in H
+  | H : no_inits <{spawn _     }> |- _ => eapply inv_noinits_spawn in H
+  end.
+
+(* lemmas ------------------------------------------------------------------ *)
+
+Corollary noinit_from_noinits : forall ad t,
+  no_inits t ->
+  no_init ad t.
+Proof.
+  unfold no_inits. auto.
+Qed.
+
+Corollary noinits_insert_term : forall t1 t2 ad t,
+  no_inits t1 ->
+  t1 --[e_insert ad t]--> t2 ->
+  no_inits t.
+Proof.
+  unfold no_inits. eauto using noinit_insert_term.
+Qed.
+
+Corollary noinits_write_term : forall t1 t2 ad t,
+  no_inits t1 ->
+  t1 --[e_write ad t]--> t2 ->
+  no_inits t.
+Proof.
+  unfold no_inits. eauto using noinit_write_term.
+Qed.
+
+(* preservation lemmas ----------------------------------------------------- *)
+
+Corollary noinits_subst : forall x tx t,
+  no_inits t ->
+  no_inits tx ->
+  no_inits <{[x := tx] t}>.
+Proof.
+  intros ** ?. eauto using noinit_subst.
+Qed.
+
