UniqueInits.v
@@ -1,0 +1,199 @@
+From Coq Require Import Lia.
+
+From Elo Require Import Core.
+From Elo Require Import Properties1.
+
+From Elo Require Import NoUninitRefs.
+From Elo Require Import OneInit.
+
+(* ------------------------------------------------------------------------- *)
+(* unique-initializers                                                       *)
+(* ------------------------------------------------------------------------- *)
+
+Definition unique_initializers (m : mem) (ths : threads) := forall ad,
+  ad < #m ->
+  (m[ad].t <> None -> forall_threads ths (no_init ad)) /\
+  (m[ad].t =  None -> forone_thread  ths (one_init ad) (no_init ad)).
+
+(* preservation lemmas ----------------------------------------------------- *)
+
+(* preservation ------------------------------------------------------------ *)
+
+Local Lemma ui_preservation_none : forall m ths tid t,
+  forall_threads ths valid_blocks ->
+  (* --- *)
+  tid < #ths ->
+  unique_initializers m ths ->
+  ths[tid] --[e_none]--> t ->
+  unique_initializers m ths[tid <- t].
+Proof.
+  intros until 1.
+  intros ? Hui ? ad Had. specialize (Hui ad Had) as [Hfall Hfone].
+  split; intros; aspecialize.
+  - intros ?. omicron; eauto using noinit_preservation_none.
+  - specialize Hfone as [tid' [? ?]]. exists tid'. split; intros; omicron;
+    eauto using noinit_preservation_none, oneinit_preservation_none.
+Qed.
+
+Local Lemma ui_preservation_alloc : forall m ths tid t T,
+  forall_threads ths (valid_addresses m) ->
+  (* --- *)
+  tid < #ths ->
+  unique_initializers m ths ->
+  ths[tid] --[e_alloc (#m) T]--> t ->
+  unique_initializers (m +++ (None, T, false)) ths[tid <- t].
+Proof.
+  intros until 1.
+  intros ? Hui ? ad Had. omicron.
+  - specialize (Hui ad) as [Hfall Hfone]; trivial.
+    split; intros; upsilon; aspecialize.
+    + intros ?. omicron; eauto using noinit_preservation_alloc.
+    + specialize Hfone as [tid' [? ?]]. exists tid'.
+      assert (ad < #m) by eauto using oneinit_ad_bound.
+      split; intros; omicron;
+      eauto using noinit_preservation_alloc, oneinit_preservation_alloc.
+  - split; intros; upsilon; auto. exists tid. split; intros; sigma;
+    eauto using noinit_from_vad, noinit_to_oneinit.
+  - lia.
+Qed.
+
+Local Lemma ui_preservation_insert : forall m ths tid t ad te,
+  forall_threads ths (valid_addresses m) ->
+  forall_threads ths valid_blocks ->
+  (* --- *)
+  tid < #ths ->
+  unique_initializers m ths ->
+  ths[tid] --[e_insert ad te]--> t ->
+  unique_initializers m[ad.t <- te] ths[tid <- t].
+Proof.
+  intros until 2.
+  intros ? Hui ? ad' Had'. sigma. specialize (Hui ad' Had') as [Hfall Hfone].
+  assert (ad < #m) by eauto using vad_insert_addr.
+  destruct (alt_opt_dec m[ad'].t); aspecialize; split; intros.
+  - specialize Hfone as [tid'' [? ?]].
+    intros tid'. repeat omicron;
+    destruct (nat_eq_dec tid'' tid'); subst;
+    eauto using oneinit_to_noinit;
+    exfalso; eauto using noinit_insert_contradiction.
+  - specialize Hfone as [tid'' [? ?]].
+    repeat omicron; try discriminate.
+    exists tid''. split; intros; omicron;
+    eauto using noinit_preservation_insert, oneinit_preservation_insert.
+  - intros tid'. repeat omicron; eauto using noinit_preservation_insert.
+    exfalso. eauto using noinit_insert_contradiction.
+  - omicron; eauto. discriminate.
+Qed.
+
+Local Lemma ui_preservation_read : forall m ths tid t ad te,
+  no_inits te ->
+  (* --- *)
+  tid < #ths ->
+  unique_initializers m ths ->
+  ths[tid] --[e_read ad te]--> t ->
+  unique_initializers m ths[tid <- t].
+Proof.
+  intros until 1.
+  intros ? Hui ? ad' Had'. specialize (Hui ad' Had') as [Hfall Hfone].
+  split; intros; upsilon; aspecialize.
+  - intros ?. omicron; eauto using noinit_preservation_read.
+  - specialize Hfone as [tid' [? ?]]. exists tid'.
+    split; intros; omicron;
+    eauto using noinit_preservation_read, oneinit_preservation_read.
+Qed.
+
+Local Lemma ui_preservation_write : forall m ths tid t ad te,
+  forall_threads ths (valid_addresses m) ->
+  forall_threads ths valid_blocks ->
+  no_uninitialized_references m ths ->
+  (* --- *)
+  tid < #ths ->
+  unique_initializers m ths ->
+  ths[tid] --[e_write ad te]--> t ->
+  unique_initializers m[ad.t <- te] ths[tid <- t].
+Proof.
+  intros until 2. intros Hnur.
+  intros ? Hui ? ad' Had'. sigma. specialize (Hui ad' Had') as [Hfall Hfone].
+  assert (ad < #m) by eauto using vad_write_addr.
+  split; intros; repeat omicron; try discriminate; try aspecialize.
+  - destruct (alt_opt_dec m[ad'].t) as [Hmad' | Hmad']; aspecialize.
+    + destruct (Hnur ad' Hmad').
+      exfalso. eauto using noref_write_contradiction.
+    + intros ?. omicron; eauto using noinit_preservation_write.
+  - intros ?. omicron; eauto using noinit_preservation_write.
+  - specialize Hfone as [tid' [? ?]]. exists tid'; split; intros;
+    omicron; eauto using noinit_preservation_write, oneinit_preservation_write.
+Qed.
+
+Local Lemma ui_preservation_acq : forall m ths tid ad t te,
+  no_inits te ->
+  (* --- *)
+  tid < #ths ->
+  unique_initializers m ths ->
+  ths[tid] --[e_acq ad te]--> t ->
+  unique_initializers m[ad.X <- true] ths[tid <- t].
+Proof.
+  intros until 1.
+  intros ? Hui ? ad' Had'. sigma. specialize (Hui ad' Had') as [Hfall Hfone].
+  split; intros; upsilon; aspecialize.
+  - intros ?. omicron; eauto using noinit_preservation_acq.
+  - specialize Hfone as [tid' [? ?]]. exists tid'.
+    split; intros; omicron;
+    eauto using noinit_preservation_acq, oneinit_preservation_acq.
+Qed.
+
+Local Lemma ui_preservation_rel : forall m ths tid ad t,
+  tid < #ths ->
+  unique_initializers m ths ->
+  ths[tid] --[e_rel ad]--> t ->
+  unique_initializers m[ad.X <- false] ths[tid <- t].
+Proof.
+  intros *.
+  intros ? Hui ? ad' Had'. sigma. specialize (Hui ad' Had') as [Hfall Hfone].
+  split; intros; upsilon; aspecialize.
+  - intros ?. omicron; eauto using noinit_preservation_rel.
+  - specialize Hfone as [tid' [? ?]]. exists tid'.
+    split; intros; omicron;
+    eauto using noinit_preservation_rel, oneinit_preservation_rel.
+Qed.
+
+Local Lemma ui_preservation_spawn : forall m ths tid t te,
+  forall_threads ths valid_blocks ->
+  (* --- *)
+  tid < #ths ->
+  unique_initializers m ths ->
+  ths[tid] --[e_spawn (#ths) te]--> t ->
+  unique_initializers m (ths[tid <- t] +++ te).
+Proof.
+  intros until 1.
+  intros ? Hui ? ad' Had'. specialize (Hui ad' Had') as [Hfall Hfone].
+  split; intros; upsilon; aspecialize.
+  - intros ?. omicron; try constructor;
+    eauto using noinit_preservation_spawn, noinit_preservation_spawned.
+  - specialize Hfone as [tid' [? ?]]. exists tid'.
+    split; intros; omicron; try constructor;
+    eauto using noinit_preservation_spawn, oneinit_preservation_spawn.
+    + invc_oneinit.
+    + eauto using noinit_spawn_term.
+Qed.
+
+Theorem ui_preservation : forall m1 m2 ths1 ths2 tid e,
+  forall_memory m1 no_inits ->
+  forall_program m1 ths1 (valid_addresses m1) ->
+  forall_program m1 ths1 valid_blocks ->
+  no_uninitialized_references m1 ths1 ->
+  (* --- *)
+  unique_initializers m1 ths1 ->
+  m1 / ths1 ~~[tid, e]~~> m2 / ths2 ->
+  unique_initializers m2 ths2.
+Proof.
+  intros * ? [? ?] [? ?] ? **. invc_cstep; try invc_mstep.
+  - eauto using ui_preservation_none.
+  - eauto using ui_preservation_alloc.
+  - eauto using ui_preservation_insert.
+  - eauto using ui_preservation_read.
+  - eauto using ui_preservation_write.
+  - eauto using ui_preservation_acq.
+  - eauto using ui_preservation_rel.
+  - eauto using ui_preservation_spawn.
+Qed.
+
