WellTypedTerm.v
@@ -96,9 +96,9 @@ Ltac invc_wtt :=
 (* auxiliary lemmas                                                          *)
 (* ------------------------------------------------------------------------- *)
 
-Lemma wtt_init_term : forall t1 t2 ad t,
+Lemma wtt_insert_term : forall t1 t2 ad t,
   well_typed_term t1 ->
-  t1 --[e_init ad t]--> t2 ->
+  t1 --[e_insert ad t]--> t2 ->
   well_typed_term t.
 Proof.
   intros. ind_tstep; invc_wtt; eauto.
