XArea.v
@@ -1,8 +1,8 @@
 From Elo Require Import Core.
+From Elo Require Import Properties1.
 
-From Elo Require Import Blocks.
-From Elo Require Import Inits.
-From Elo Require Import CriticalRegions.
+From Elo Require Import UniqueInits.
+From Elo Require Import ConsistentInits.
 
 (* ------------------------------------------------------------------------- *)
 (* init-cr-exclusivity                                                       *)
@@ -22,8 +22,57 @@ Lemma ice_preservation_none : forall m ths tid t,
   init_cr_exclusivity m ths[tid <- t].
 Proof.
   intros * ? Hice ? ad tid1 tid2.
-  specialize (Hice ad tid1 tid2) as [? ?].
-  split; intros; repeat omicron;
+  destruct (Hice ad tid1 tid2) as [? ?].
+  split; intros; repeat omicron; auto;
   eauto using nocr_preservation_none, oneinit_inheritance_none;
   eauto using noinit_preservation_none, onecr_inheritance_none.
+Qed.
+
+Lemma ice_preservation_alloc : forall m ths tid t T,
+  forall_threads ths (valid_addresses m) ->
+  forall_threads ths valid_blocks ->
+  (* --- *)
+  init_cr_exclusivity m ths ->
+  ths[tid] --[e_alloc (#m) T]--> t ->
+  init_cr_exclusivity (m +++ (None, T, false)) ths[tid <- t].
+Proof.
+  intros * Hvad ? Hice ? ad tid1 tid2.
+  destruct (Hice ad tid1 tid2) as [? ?].
+  assert (forall tid, no_cr (#m) ths[tid]) by eauto using nocr_from_vad.
+  split; intros; repeat omicron; auto; destruct (nat_eq_dec ad (#m)); subst;
+  eauto using nocr_preservation_alloc, oneinit_inheritance_alloc;
+  eauto using noinit_preservation_alloc, onecr_inheritance_alloc;
+  exfalso; eauto using onecr_inheritance_alloc, nocr_onecr_contradiction.
+Qed.
+
+Theorem insert_then_noinit : forall m ths tid t ad te,
+  forall_threads ths (valid_addresses m) ->
+  forall_threads ths (consistent_inits m) ->
+  unique_initializers m ths ->
+  (* --- *)
+  ths[tid] --[e_insert ad te]--> t ->
+  one_init ad ths[tid].
+Proof.
+  intros * ? ? Hui **.
+  assert (Had   : ad < #m) by eauto using vad_insert_addr.
+  assert (Hnone : m[ad].t = None) by eauto using insert_then_uninitialized.
+  specialize (Hui ad Had) as [_ Hui]. specialize (Hui Hnone) as [tid' [? ?]].
+  destruct (nat_eq_dec tid' tid); subst; trivial.
+  exfalso. eauto using noinit_insert_contradiction.
+Qed.
+
+Lemma ice_preservation_insert : forall m ths tid t ad te,
+  forall_threads ths valid_blocks ->
+  (* --- *)
+  init_cr_exclusivity m ths ->
+  ths[tid] --[e_insert ad te]--> t ->
+  init_cr_exclusivity m ths[tid <- t].
+Proof.
+  intros until 1. rename ad into ad'.
+  intros Hice ? ad tid1 tid2.
+  destruct (Hice ad tid1 tid2) as [? ?].
+  split; intros; repeat omicron; auto; destruct (nat_eq_dec ad' ad); subst;
+  eauto using nocr_preservation_insert, oneinit_inheritance_insert;
+  eauto using noinit_preservation_insert, onecr_inheritance_insert.
+  -
 Qed.
